Tainted typing

lambda2Gmu/Definitions.v
@@ -903,7 +903,7 @@ Inductive wft : GADTEnv -> typctx -> typ -> Prop :=
 .
 
 (*Thanks to usage of de Bruijn indices, alpha equivalence reduces to plain equivalence *)
-Definition alpha_equivalent (T U : typ) : Prop := T = U.
+(* Definition alpha_equivalent (T U : typ) : Prop := T = U. *)
 
 Fixpoint subst_tt' (T : typ) (Θ : substitution) :=
   match Θ with
@@ -939,7 +939,7 @@ Inductive subst_matches_typctx Σ : typctx -> substitution -> Prop :=
     subst_matches_typctx Σ (tc_var A :: Δ) ((A, T) :: Θ)
 | tc_add_eq : forall Θ Δ T1 T2,
     subst_matches_typctx Σ Δ Θ ->
-    alpha_equivalent (subst_tt' T1 Θ) (subst_tt' T2 Θ) ->
+    (subst_tt' T1 Θ) = (subst_tt' T2 Θ) ->
     subst_matches_typctx Σ (tc_eq (T1 ≡ T2) :: Δ) Θ.
 
 (* Semantic entailment of a set of equations, noted in the paper as Δ ⊨ T1 ≡ T2.
@@ -949,7 +949,7 @@ Definition entails_semantic Σ (Δ : typctx) (eq : type_equation) :=
   match eq with
   | T1 ≡ T2 =>
     forall Θ, subst_matches_typctx Σ Δ Θ ->
-         alpha_equivalent (subst_tt' T1 Θ) (subst_tt' T2 Θ)
+         (subst_tt' T1 Θ) = (subst_tt' T2 Θ)
   end.
 
 (* a shorthand allowing to define a list of free vars in Δ *)
@@ -1050,20 +1050,24 @@ Inductive okt : GADTEnv -> typctx -> ctx -> Prop :=
 Definition equations_from_lists Ts Us : typctx :=
   zipWith (fun U V : typ => tc_eq (U ≡ V)) Ts Us.
 
-Reserved Notation "{ Σ , Δ ,  E }  ⊢ t ∈ T" (at level 0, Σ at level 99, T at level 69).
+Reserved Notation "{ Σ , Δ ,  E }  ⊢( L ) t ∈ T" (at level 0, Σ at level 99, T at level 69).
 
-Inductive typing : GADTEnv -> typctx -> ctx -> trm -> typ -> Prop :=
+Inductive typing_taint : Set :=
+| Treg
+| Teq.
+
+Inductive typing : typing_taint -> GADTEnv -> typctx -> ctx -> trm -> typ -> Prop :=
   (* TODO typing_eq *)
 | typing_unit : forall Σ Δ E,
     okt Σ Δ E ->
-    {Σ, Δ, E} ⊢ trm_unit ∈ typ_unit
+    {Σ, Δ, E} ⊢(Treg) trm_unit ∈ typ_unit
 | typing_var : forall Σ E Δ x T,
     binds x (bind_var T) E ->
     okt Σ Δ E ->
-    {Σ, Δ, E} ⊢ (trm_fvar x) ∈ T (* x: T ⊢ x: T *)
-| typing_cons : forall Σ E Δ Ts Name Ctor e1 Tarity Ctors Carity CargType CretTypes Targ Tret,
+    {Σ, Δ, E} ⊢(Treg) (trm_fvar x) ∈ T (* x: T ⊢ x: T *)
+| typing_cons : forall Σ E Δ TT1 Ts Name Ctor e1 Tarity Ctors Carity CargType CretTypes Targ Tret,
     (* to typecheck the constructor: *)
-    {Σ, Δ, E} ⊢ e1 ∈ Targ -> (* we need to typecheck its only data parameter - its typ must match the argument type (see below) *)
+    {Σ, Δ, E} ⊢(TT1) e1 ∈ Targ -> (* we need to typecheck its only data parameter - its typ must match the argument type (see below) *)
     binds Name (mkGADT Tarity Ctors) Σ -> (* the GADT called `Name` that we are building must be bound in the Σ env and we check its constructors and arity *)
     nth_error Ctors Ctor = Some (mkGADTconstructor Carity CargType CretTypes) -> (* we specify that we construct the constructor with id Ctor, so we need to check that such constructor really exists and get its definition from the Ctors list *)
     length Ts = Carity -> (* the amount of concrete type parameters that we are instantiating the constructor with must be equal to the constructor's arity *)
@@ -1071,47 +1075,47 @@ Inductive typing : GADTEnv -> typctx -> ctx -> trm -> typ -> Prop :=
     (forall T, In T Ts -> wft Σ Δ T) -> (* the concrete type parameters that we are instantiating the constructor with must be well formed in the current environment *)
     (* alternatively: Tret = open_tt_many (typ_gadt (List.map (fun T => open_tt_many T Ts) CretTypes) Name) Ts -> *)
     Tret = open_tt_many Ts (typ_gadt CretTypes Name) -> (* as with the argument, the types that will be in the type of the returned GADT must also be opened with the type parameters *)
-    {Σ, Δ, E} ⊢ trm_constructor Ts (Name, Ctor) e1 ∈ Tret
-| typing_abs : forall L Σ Δ E V e1 T1,
-    (forall x, x \notin L -> {Σ, Δ, E & x ~: V} ⊢ e1 open_ee_var x ∈ T1) ->
-    {Σ, Δ, E} ⊢ trm_abs V e1 ∈ V ==> T1
-| typing_app : forall Σ Δ E T1 T2 e1 e2,
-    {Σ, Δ, E} ⊢ e2 ∈ T1 ->
-    {Σ, Δ, E} ⊢ e1 ∈ T1 ==> T2 ->
-    {Σ, Δ, E} ⊢ trm_app e1 e2 ∈ T2
-| typing_tabs : forall L Σ Δ E e1 T1,
+    {Σ, Δ, E} ⊢(Treg) trm_constructor Ts (Name, Ctor) e1 ∈ Tret
+| typing_abs : forall L Σ Δ E V e1 T1 TT,
+    (forall x, x \notin L -> {Σ, Δ, E & x ~: V} ⊢(TT) e1 open_ee_var x ∈ T1) ->
+    {Σ, Δ, E} ⊢(Treg) trm_abs V e1 ∈ V ==> T1
+| typing_app : forall Σ Δ E T1 T2 e1 e2 TT1 TT2,
+    {Σ, Δ, E} ⊢(TT1) e2 ∈ T1 ->
+    {Σ, Δ, E} ⊢(TT2) e1 ∈ T1 ==> T2 ->
+    {Σ, Δ, E} ⊢(Treg) trm_app e1 e2 ∈ T2
+| typing_tabs : forall L Σ Δ E e1 T1 TT,
     (forall X, X \notin L -> (* TODO consider splitting value and term as this case may be problematic ? *)
           value (e1 open_te_var X)) ->
     (forall X, X \notin L ->
-          {Σ, Δ |,| [tc_var X], E} ⊢ (e1 open_te_var X) ∈ (T1 open_tt_var X)) ->
-    {Σ, Δ, E} ⊢ (trm_tabs e1) ∈ typ_all T1
-| typing_tapp : forall Σ Δ E e1 T1 T T',
-    {Σ, Δ, E} ⊢ e1 ∈ typ_all T1 ->
+          {Σ, Δ |,| [tc_var X], E} ⊢(TT) (e1 open_te_var X) ∈ (T1 open_tt_var X)) ->
+    {Σ, Δ, E} ⊢(Treg) (trm_tabs e1) ∈ typ_all T1
+| typing_tapp : forall Σ Δ E e1 T1 T T' TT,
+    {Σ, Δ, E} ⊢(TT) e1 ∈ typ_all T1 ->
     wft Σ Δ T -> (* corresponds to the check `Δ; Γ ⊢ τ1 : *` *)
     T' = open_tt T1 T ->
-    {Σ, Δ, E} ⊢ trm_tapp e1 T ∈ T'
-| typing_tuple : forall Σ Δ E T1 T2 e1 e2,
-    {Σ, Δ, E} ⊢ e1 ∈ T1 ->
-    {Σ, Δ, E} ⊢ e2 ∈ T2 ->
-    {Σ, Δ, E} ⊢ trm_tuple e1 e2 ∈ T1 ** T2
-| typing_fst : forall Σ Δ E T1 T2 e1,
-    {Σ, Δ, E} ⊢ e1 ∈ T1 ** T2 ->
-    {Σ, Δ, E} ⊢ trm_fst e1 ∈ T1
-| typing_snd : forall Σ Δ E T1 T2 e1,
-    {Σ, Δ, E} ⊢ e1 ∈ T1 ** T2 ->
-    {Σ, Δ, E} ⊢ trm_snd e1 ∈ T2
-| typing_fix : forall L Σ Δ E T v,
+    {Σ, Δ, E} ⊢(Treg) trm_tapp e1 T ∈ T'
+| typing_tuple : forall Σ Δ E T1 T2 e1 e2 TT1 TT2,
+    {Σ, Δ, E} ⊢(TT1) e1 ∈ T1 ->
+    {Σ, Δ, E} ⊢(TT2) e2 ∈ T2 ->
+    {Σ, Δ, E} ⊢(Treg) trm_tuple e1 e2 ∈ T1 ** T2
+| typing_fst : forall Σ Δ E T1 T2 e1 TT,
+    {Σ, Δ, E} ⊢(TT) e1 ∈ T1 ** T2 ->
+    {Σ, Δ, E} ⊢(Treg) trm_fst e1 ∈ T1
+| typing_snd : forall Σ Δ E T1 T2 e1 TT,
+    {Σ, Δ, E} ⊢(TT) e1 ∈ T1 ** T2 ->
+    {Σ, Δ, E} ⊢(Treg) trm_snd e1 ∈ T2
+| typing_fix : forall L Σ Δ E T v TT,
     (forall x, x \notin L -> value (v open_ee_var x)) ->
-    (forall x, x \notin L -> {Σ, Δ, E & x ~: T} ⊢ (v open_ee_var x) ∈ T) ->
-    {Σ, Δ, E} ⊢ trm_fix T v ∈ T
-| typing_let : forall L Σ Δ E V T2 e1 e2,
-    {Σ, Δ, E} ⊢ e1 ∈ V ->
-    (forall x, x \notin L -> {Σ, Δ, E & x ~: V} ⊢ e2 open_ee_var x ∈ T2) ->
-    {Σ, Δ, E} ⊢ trm_let e1 e2 ∈ T2
+    (forall x, x \notin L -> {Σ, Δ, E & x ~: T} ⊢(TT) (v open_ee_var x) ∈ T) ->
+    {Σ, Δ, E} ⊢(Treg) trm_fix T v ∈ T
+| typing_let : forall L Σ Δ E V T2 e1 e2 TT1 TT2,
+    {Σ, Δ, E} ⊢(TT1) e1 ∈ V ->
+    (forall x, x \notin L -> {Σ, Δ, E & x ~: V} ⊢(TT2) e2 open_ee_var x ∈ T2) ->
+    {Σ, Δ, E} ⊢(Treg) trm_let e1 e2 ∈ T2
 (* typing case merges rules ty-case and pat-cons from the original paper *)
 (* for example, let's see we are typing the match as in the eval function defined above; since there are many branches, we will look at the Pair branch in particular *)
-| typing_case : forall L Σ Δ E e ms Ts T Name Tc Tarity Defs,
-    {Σ, Δ, E} ⊢ e ∈ T -> (* first we need to typecheck the expression that we will be matching, in our eval example it is the argument that we are matching *)
+| typing_case : forall L Σ Δ E e ms Ts T Name Tc Tarity Defs TT1,
+    {Σ, Δ, E} ⊢(TT1) e ∈ T -> (* first we need to typecheck the expression that we will be matching, in our eval example it is the argument that we are matching *)
     T = (typ_gadt Ts Name) -> (* for the match to work, that expression must be a GADT and its name must match the one that is provided in the syntax, in our example `Expr` *)
     binds Name (mkGADT Tarity Defs) Σ -> (* that GADT must be bound in our Σ environment *)
     length Defs = length ms -> (* implicit exhaustivity check: our pattern match must have as many branches as the GADT we are matching has constructors since we have a 1-1 correspondence between branches and constructors; in our case there are 4 branches *)
@@ -1121,7 +1125,9 @@ Inductive typing : GADTEnv -> typctx -> ctx -> trm -> typ -> Prop :=
                    (* we need to make sure that the arity defined in the syntax actually matches the arity of the respective constructor,
                       in our example we check that the match brings two type variables [X,Y] and the arity of the Pair constructor is 2 *)
                    clauseArity clause = Carity def) ->
-    (forall def clause, In (def, clause) (zip Defs ms) -> (* now, for each pair of: constructor definition + a clause matching that constructor, we check the actual important properties: *)
+    (forall def clause, In (def, clause) (zip Defs ms) ->
+                   exists TTc, (* each inner clause can have a different taint so we account for that *)
+                   (* now, for each pair of: constructor definition + a clause matching that constructor, we check the actual important properties: *)
                forall Alphas x,
                  length Alphas = Carity def -> (* since we instantiate the type variables, we need to ensure that the added type variables amount is equalt to the arity *)
                  (* below follow multiple freshness conditions that boil down to: Alphas and x are fresh and mutually distinct *)
@@ -1149,14 +1155,14 @@ Inductive typing : GADTEnv -> typctx -> ctx -> trm -> typ -> Prop :=
                    (* Ts === Crettypes def; in our example that equation is X ** Y =:= A *)
                    E
                    & x ~: (open_tt_many_var Alphas (Cargtype def)) (* e: [X]Expr ** [Y]Expr *)
-                 } ⊢ (open_te_many_var Alphas (clauseTerm clause)) open_ee_var x ∈ Tc
+                 } ⊢(TTc) (open_te_many_var Alphas (clauseTerm clause)) open_ee_var x ∈ Tc
             ) ->
-    { Σ, Δ, E } ⊢ trm_matchgadt e Name ms ∈ Tc
-| typing_eq : forall Σ Δ E T1 T2 e,
-    { Σ, Δ, E } ⊢ e ∈ T1 ->
+    { Σ, Δ, E } ⊢(Treg) trm_matchgadt e Name ms ∈ Tc
+| typing_eq : forall Σ Δ E T1 T2 e TT,
+    { Σ, Δ, E } ⊢(TT) e ∈ T1 ->
     entails_semantic Σ Δ (T1 ≡ T2) ->
-    { Σ, Δ, E } ⊢ e ∈ T2
-where "{ Σ , Δ , E } ⊢ t ∈ T" := (typing Σ Δ E t T).
+    { Σ, Δ, E } ⊢(Teq) e ∈ T2
+where "{ Σ , Δ , E } ⊢( R ) t ∈ T" := (typing R Σ Δ E t T).
 
 (** * Reduction rules (Small-step operational semantics) *)
 
@@ -1254,11 +1260,11 @@ where "e1 --> e2" := (red e1 e2).
 
 (** * Statemenf of desired safety properties *)
 
-Definition progress := forall Σ e T,
-    {Σ, emptyΔ, empty} ⊢ e ∈ T ->
+Definition progress := forall TT Σ e T,
+    {Σ, emptyΔ, empty} ⊢(TT) e ∈ T ->
     (value e) \/ (exists e', e --> e').
 
-Definition preservation := forall Σ e T e',
-    {Σ, emptyΔ, empty} ⊢ e ∈ T ->
+Definition preservation := forall TT1 TT2 Σ e T e',
+    {Σ, emptyΔ, empty} ⊢(TT1) e ∈ T ->
     e --> e' ->
-    {Σ, emptyΔ, empty} ⊢ e' ∈ T.
+    {Σ, emptyΔ, empty} ⊢(TT2) e' ∈ T.
