lambda2Gmu/CanonicalForms.v
@@ -8,21 +8,18 @@ Require Import TLC.LibLN.
 (* TODO add assumptions that Δ is not contradictory *)
   (* Ht : {Σ, empty}⊢ trm_constructor Tparams Name e1 ∈ T1 ** T2 *)
 Lemma CanonicalConstructorType : forall Σ Δ E Tparams Name Ctor e1 T,
-    {Σ, Δ, E} ⊢ trm_constructor Tparams (Name, Ctor) e1 ∈ T ->
-    ~ (contradictory_bounds Σ Δ) ->
+    {Σ, Δ, E} ⊢(Treg) trm_constructor Tparams (Name, Ctor) e1 ∈ T ->
     (* TODO can we make Typs more specific? *)
     exists Typs, T = typ_gadt Typs Name.
-  introv Htyp Hbound.
+  introv Htyp.
   inversions Htyp.
-  - rewrite rewrite_open_tt_many_gadt.
-    eexists.
-    f_equal.
-  - destruct T.
-Admitted.
+  rewrite rewrite_open_tt_many_gadt.
+  eexists.
+  f_equal.
+Qed.
 
 Lemma CanonicalConstructorTypeGen : forall Σ Δ E Tparams Ctor e1 T,
-    {Σ, Δ, E} ⊢ trm_constructor Tparams Ctor e1 ∈ T ->
-    ~ (contradictory_bounds Σ Δ) ->
+    {Σ, Δ, E} ⊢(Treg) trm_constructor Tparams Ctor e1 ∈ T ->
     (* TODO can we make Typs more specific? *)
     exists Typs Name, T = typ_gadt Typs Name.
   intros.
@@ -32,11 +29,11 @@ Lemma CanonicalConstructorTypeGen : forall Σ Δ E Tparams Ctor e1 T,
   eexists. eexists. eauto.
 Qed.
 
-#[export] Hint Resolve CanonicalConstructorTypeGen.
+Local Hint Resolve CanonicalConstructorTypeGen.
 
 Ltac contradictory_constructor_type :=
   lazymatch goal with
-  | H: {?S, ?D, ?E} ⊢ trm_constructor ?Ts ?C ?e ∈ ?T |- _ =>
+  | H: {?S, ?D, ?E} ⊢(?TT) trm_constructor ?Ts ?C ?e ∈ ?T |- _ =>
     apply CanonicalConstructorTypeGen in H;
     let Hcontradict := fresh "contradict" in
     destruct H as [? [? Hcontradict]];
@@ -45,48 +42,48 @@ Ltac contradictory_constructor_type :=
 
 Lemma CanonicalFormTuple : forall Σ Δ E e T1 T2,
     value e ->
-    {Σ, Δ, E} ⊢ e ∈ T1 ** T2 ->
+    {Σ, Δ, E} ⊢(Treg) e ∈ T1 ** T2 ->
     exists v1 v2, e = trm_tuple v1 v2.
   introv Hv Ht.
   inversion Hv; inversion Ht; subst; eauto; try congruence.
-  (* contradictory_constructor_type. *)
-Admitted.
+  contradictory_constructor_type.
+Qed.
 
 Lemma CanonicalFormAbs : forall Σ Δ E e T1 T2,
     value e ->
-    {Σ, Δ, E} ⊢ e ∈ T1 ==> T2 ->
+    {Σ, Δ, E} ⊢(Treg) e ∈ T1 ==> T2 ->
     exists v1, e = trm_abs T1 v1.
   introv Hv Ht.
   inversion Hv; inversion Ht; subst; eauto; try congruence.
-  (* contradictory_constructor_type. *)
-Admitted.
+  contradictory_constructor_type.
+Qed.
 
 Lemma CanonicalFormTAbs : forall Σ Δ E e T,
     value e ->
-    {Σ, Δ, E} ⊢ e ∈ typ_all T ->
+    {Σ, Δ, E} ⊢(Treg) e ∈ typ_all T ->
     exists v1, e = trm_tabs v1.
   introv Hv Ht.
   inversion Hv; inversion Ht; subst; eauto; try congruence.
-  (* contradictory_constructor_type. *)
-Admitted.
+  contradictory_constructor_type.
+Qed.
 
 Lemma CanonicalFormUnit : forall Σ Δ E e,
     value e ->
-    {Σ, Δ, E} ⊢ e ∈ typ_unit ->
+    {Σ, Δ, E} ⊢(Treg) e ∈ typ_unit ->
     e = trm_unit.
   introv Hv Ht.
   inversion Hv; inversion Ht; subst; eauto; try congruence.
-  (* contradictory_constructor_type. *)
-Admitted.
+  contradictory_constructor_type.
+Qed.
 
 Lemma CanonicalFormGadt : forall Σ Δ E e Ts N,
     value e ->
-    {Σ, Δ, E} ⊢ e ∈ typ_gadt Ts N ->
+    {Σ, Δ, E} ⊢(Treg) e ∈ typ_gadt Ts N ->
     exists Ts' C v, e = trm_constructor Ts' (N, C) v. (* todo may want to relate Ts' to Ts *)
   introv Hv Ht.
   inversion Hv; inversion Ht; subst; eauto; try congruence.
-  (* rewrite rewrite_open_tt_many_gadt in H8. *)
-  (* inversions H8. *)
-  (* inversions H12. *)
-  (* repeat eexists. *)
-Admitted.
+  rewrite rewrite_open_tt_many_gadt in H8.
+  inversions H8.
+  inversions H13.
+  repeat eexists.
+Qed.
